# RealApp

رابطه بازگشتی زیر را به وسیله حل معادله حل کنید؟

$$\left\{     \begin{array}{1}     a_n = 4a_{n-1} - 4a_{n-2} \\     a_0 = 1 ; a_1=4     \end{array}     \right.$$

$$\rightarrow      n^2-4n+4=0     \rightarrow     \Delta = b^2-4a*c==16-4*1*4=0\\     \rightarrow      \frac{-b}{2a}     \rightarrow     \frac{4}{2}=2$$

روش دوم:

(x-2)(x-2)=0→x-2==x=2;x-2==x=2

به روش دستگاه:

$$(\alpha_1 + \alpha_2n)2^n\\     \rightarrow     \alpha_1=1 , 2^1(\alpha_1+\alpha_2)=4     \rightarrow     2+2\alpha_2=4     \rightarrow     2\alpha_2=2     \rightarrow     \alpha_2=1\\     \rightarrow     (1+h)2^n=2^n+n2^n     \rightarrow \theta(n2^n)$$

رابطه بازگشتی زیر را به وسیله حل معادله حل کنید؟

$$\left\{     \begin{array}{1}     a_n = 3a_n-1 - 2a_n-2 \\     a_0 = 1 ; a_1=2     \end{array}     \right.$$

$$\rightarrow x^2-3x-2=0     \rightarrow      \Delta= b^2-4a*c==16-4*1*4=0\\     \rightarrow      \frac{-b\pm\sqrt{\Delta}}{2a}     \rightarrow     \frac{3+1}{2}=2,     \frac{3-1}{2}=1$$

به روش دستگاه:

$$(\alpha_1*2^n+\alpha_2*1^n)     \rightarrow\\     \alpha_1+\alpha_2=1\\     -2\alpha_1+\alpha_2=-2\\     \rightarrow\alpha_1=1$$

رابطه بازگشتی زیر را به وسیله حل معادله حل کنید؟

$$a_n=a_n-1+n\\     \rightarrow(x-1)(x-1)^2=0 \rightarrow x-1=0,x=1\\     \rightarrow (\alpha_1+\alpha_2n+\alpha_3n^2)^n\\     \theta(n^2)$$

رابطه بازگشتی زیر را به وسیله حل معادله حل کنید؟

$$a_{n+1} = 4a_{n-1} +2^{n+3}+n*2^n\\     \rightarrow 2^n(2^3+n) \rightarrow 2^n(n+1)\\     \rightarrow (x^2-4)(x-2)^2=0\\     \rightarrow x^2-4=0 \rightarrow x2=\Delta=\pm2,(x-2)^2=0\rightarrow n=2\\     \rightarrow (\alpha_1+\alpha_2n+\alpha_3n^2)2^n+\alpha_4(-2)n\rightarrow if\alpha_3=\not0\\     \theta(n^22^n)$$

رابطه بازگشتی زیر را به وسیله حل معادله حل کنید؟

$$a_n=3(n-1)a_{n-2}+2(n-2)a_{n-1}\\     a_0=a_1=4\\     \rightarrow n=a_n=b_n\rightarrow an=\frac{b_n}{n},b_n=3b_{n-1}-2b_{n}-2\\     \rightarrow x^2-3n+2=0,\Delta=b^2-4a*c==9-8=1,x=\frac{-b\pm\sqrt{\Delta}}{2a}=\frac{-3\pm1}{2}=2,1\\     \frac{\alpha_12^n+\alpha_21^n}{n}\rightarrow \theta(\frac{2^n}{n})$$

رابطه بازگشتی زیر را به وسیله حل معادله حل کنید؟

$$a_n=a_{n-1}*a^2_{n-2}\\     \rightarrow \log a_n=log a_{n-1}+log a^2_{n-2}\\     \rightarrow log a_n = log a_{n-1}+2loga_{n-2} \rightarrow log a_n =b_n\rightarrow b_n=b_{n-1}+2logb_{n-2}$$



